Added new rules mem_solver, strg_solver, and jumpi_eval. Extended snd results with is_sat and is_safe_cmp premises

optimizations/jumpi_eval.v
@@ -2,6 +2,8 @@ Require Import bbv.Word.
 Require Import Nat. 
 Require Import Coq.NArith.NArith.
 
+Require Import Coq.Logic.FunctionalExtensionality.
+
 Require Import FORVES2.constants.
 Import Constants.
 
@@ -57,11 +59,21 @@ Require Import List.
 Import ListNotations.
 
 
-Module Opt_div_one.
+Module Opt_jumpi_eval.
 
 
-(* DIV(X,1) = X *)
-Definition optimize_div_one_sbinding : opt_smap_value_type := 
+Definition val_diff_zero (arg: sstack_val) (fcmp: sstack_val_cmp_t) 
+  (maxid: nat) (sb: sbindings) (ctx: constraints) (ops: stack_op_instr_map) 
+  : bool :=
+match follow_in_smap arg maxid sb with
+  | Some (FollowSmapVal (SymBasicVal (Val v)) _ _) => 
+      negb (weqb v WZero)
+  | _ => false
+  end.
+
+
+(* JUMPI(Dest,B) = Dest if B is constant and B <> 0 *)
+Definition optimize_jumpi_eval_sbinding : opt_smap_value_type := 
 fun (val: smap_value) =>
 fun (fcmp: sstack_val_cmp_t) =>
 fun (sb: sbindings) =>
@@ -69,8 +81,8 @@ fun (maxid: nat) =>
 fun (ctx: constraints) =>
 fun (ops: stack_op_instr_map) => 
 match val with
-| SymOp DIV [arg1; arg2] => 
-  if fcmp ctx arg2 (Val WOne) maxid sb maxid sb ops then
+| SymOp JUMPI [arg1; arg2] => 
+  if val_diff_zero arg2 fcmp maxid sb ctx ops then
     (SymBasicVal arg1, true)
   else
     (val, false)
@@ -78,72 +90,63 @@ match val with
 end.
 
 
-
-
-
-
-Lemma optimize_div_one_sbinding_smapv_valid:
-opt_smapv_valid_snd optimize_div_one_sbinding.
+Lemma optimize_jumpi_eval_sbinding_smapv_valid:
+opt_smapv_valid_snd optimize_jumpi_eval_sbinding.
 Proof.
 unfold opt_smapv_valid_snd.
 intros ctx n fcmp sb val val' flag.
 intros _ _ Hvalid_smapv_val Hvalid_sb Hoptm_sbinding.
-unfold optimize_div_one_sbinding in Hoptm_sbinding.
+unfold optimize_jumpi_eval_sbinding in Hoptm_sbinding.
 destruct (val) as [basicv|pushtagv|label args|offset smem|key sstrg|
-  offset size smem] eqn: eq_val; try (
-    injection Hoptm_sbinding as eq_val' eq_flag;
-    rewrite <- eq_val';
-    assumption).
-destruct label eqn: eq_label; try 
-      (injection Hoptm_sbinding as eq_val' eq_flag;
-      rewrite <- eq_val'; assumption).
-(* DIV *)
-destruct args as [|arg1 r1] eqn: eq_args; try 
-  (injection Hoptm_sbinding as eq_val' eq_flag;
-  rewrite <- eq_val'; assumption).
-destruct r1 as [|arg2 r2] eqn: eq_r1; try 
-  (injection Hoptm_sbinding as eq_val' eq_flag;
-  rewrite <- eq_val'; assumption).
-destruct r2 as [|arg3 r3] eqn: eq_r2; try 
-  (injection Hoptm_sbinding as eq_val' eq_flag;
-  rewrite <- eq_val'; assumption).
-destruct (fcmp ctx arg2 (Val WOne) n sb n sb evm_stack_opm) 
-    eqn: eq_fcmp_arg2; try (injection Hoptm_sbinding as eq_val' eq_flag;
-    rewrite <- eq_val'; assumption).
-  injection Hoptm_sbinding as eq_val' eq_flag.
+  offset size smem] eqn: eq_val; 
+   try inject_rw Hoptm_sbinding eq_val'.
+destruct label eqn: eq_label; try inject_rw Hoptm_sbinding eq_val'. try 
+(* JUMPI *)
+destruct args as [|arg1 r1] eqn: eq_args; try inject_rw Hoptm_sbinding eq_val'.
+destruct r1 as [|arg2 r2] eqn: eq_r1; try inject_rw Hoptm_sbinding eq_val'.
+destruct r2 as [|arg3 r3] eqn: eq_r2; try inject_rw Hoptm_sbinding eq_val'.
+destruct (val_diff_zero arg2 fcmp n sb ctx evm_stack_opm)
+  eqn: eq_val_diff_zero_arg1.
+* injection Hoptm_sbinding as eq_val' eq_flag.
   rewrite <- eq_val'.
   simpl in Hvalid_smapv_val. unfold valid_stack_op_instr in Hvalid_smapv_val.
   simpl in Hvalid_smapv_val.
   destruct Hvalid_smapv_val as [_ [Hvalid_arg1 [Hvalid_arg2 _]]].
   simpl.
   assumption.
+* injection Hoptm_sbinding as eq_val' eq_flag.
+  rewrite <- eq_val'.
+  assumption.
 Qed.
 
 
-Lemma evm_div_one: forall ctx (x: EVMWord), evm_div ctx [x; WOne] = x.
+
+Lemma evm_jumpi_not_zero: forall exts a b,
+weqb b WZero = false ->
+evm_jumpi exts [a; b] = a.
 Proof.
-intros. simpl. unfold wdiv. unfold wordBin. simpl. 
-rewrite -> N.div_1_r. rewrite -> NToWord_wordToN.
+intros exts a b Hb_not_z. simpl.
+rewrite -> Hb_not_z.
 reflexivity.
 Qed.
 
 
-Lemma optimize_div_one_sbinding_snd:
-opt_sbinding_snd optimize_div_one_sbinding.
+Lemma optimize_jumpi_eval_sbinding_snd:
+opt_sbinding_snd optimize_jumpi_eval_sbinding.
 Proof.
 unfold opt_sbinding_snd.
 intros val val' fcmp sb maxidx ctx idx flag Hsafe_sstack_val_cmp
-  Hvalid Hissat Hoptm_sbinding.
+  Hvalid His_sat Hoptm_sbinding.
 split.
 - (* valid_sbindings *)
-  apply valid_bindings_snd_opt with (val:=val)(opt:=optimize_div_one_sbinding)
+  apply valid_bindings_snd_opt with (val:=val)(opt:=optimize_jumpi_eval_sbinding)
     (fcmp:=fcmp)(flag:=flag)(ctx:=ctx); try assumption.
-  apply optimize_div_one_sbinding_smapv_valid. 
+  apply optimize_jumpi_eval_sbinding_smapv_valid. 
     
 - (* evaluation is preserved *) 
-  intros model mem strg ext v Hismodel Heval_orig.
-  unfold optimize_div_one_sbinding in Hoptm_sbinding.
-  pose proof (Hvalid_maxidx maxidx idx val sb evm_stack_opm
+  intros model mem strg exts v His_model Heval_orig.
+  unfold optimize_jumpi_eval_sbinding in Hoptm_sbinding.
+  pose proof (Hvalid_maxidx  maxidx idx val sb evm_stack_opm
       Hvalid) as eq_maxidx_idx.
   destruct val as [vv|vv|label args|offset smem|key sstrg|offset seze smem]
     eqn: eq_val; try inject_rw Hoptm_sbinding eq_val'.
@@ -155,18 +158,19 @@ split.
     try inject_rw Hoptm_sbinding eq_val'.
   destruct r2 as [|arg3 r3] eqn: eq_r2; 
     try inject_rw Hoptm_sbinding eq_val'.
-  destruct (fcmp ctx arg2 (Val WOne) idx sb idx sb) 
-    eqn: fcmp_arg2_one.
-  + (* arg2 ~ One *)
+  destruct (val_diff_zero arg2 fcmp idx sb ctx evm_stack_opm) 
+    eqn: eq_val_diff_z_arg2.
+  + (* arg2  <> WZero *)
     injection Hoptm_sbinding as eq_val' _. 
     rewrite <- eq_val'.
     unfold eval_sstack_val in Heval_orig. simpl in Heval_orig.
     rewrite -> PeanoNat.Nat.eqb_refl in Heval_orig.
     simpl in Heval_orig.
-    destruct (eval_sstack_val' maxidx arg1 model mem strg ext idx sb evm_stack_opm)
+    destruct (eval_sstack_val' maxidx arg1 model mem strg exts idx sb evm_stack_opm)
       as [varg1|] eqn: eval_arg1; try discriminate.
-    destruct (eval_sstack_val' maxidx arg2 model mem strg ext idx sb evm_stack_opm)
+    destruct (eval_sstack_val' maxidx arg2 model mem strg exts idx sb evm_stack_opm)
       as [varg2|] eqn: eval_arg2; try discriminate.
+    unfold safe_sstack_val_cmp in Hsafe_sstack_val_cmp.
 
     unfold valid_bindings in Hvalid.
     destruct Hvalid as [eq_maxid [Hvalid_smap_value Hvalid_bindings_sb]].
@@ -176,34 +180,33 @@ split.
     destruct (Hvalid_smap_value) as [_ [Hvalid_arg1 [Hvalid_arg2 _ ]]].
     fold valid_bindings in Hvalid_bindings_sb.
 
-    pose proof (valid_sstack_value_const idx v) as 
-      Hvalid_v.
-    pose proof (Hsafe_sstack_val_cmp ctx arg2 (Val WOne) idx sb idx sb 
-      evm_stack_opm Hissat Hvalid_arg2 Hvalid_v Hvalid_bindings_sb
-      Hvalid_bindings_sb fcmp_arg2_one model mem strg ext Hismodel)
-      as [vone [Heval_arg2 Heval_vone]].
-      
-    unfold eval_sstack_val in Heval_vone.
-    rewrite -> eval_sstack_val'_const in Heval_vone.
-    rewrite <- Heval_vone in Heval_arg2.
-    unfold eval_sstack_val in Heval_arg2.
-    rewrite -> eq_maxidx_idx in Heval_arg2.
-    rewrite -> Heval_arg2 in eval_arg2.
-    injection eval_arg2 as eq_varg2.
-    rewrite <- eq_varg2 in Heval_orig.
-    rewrite -> evm_div_one in Heval_orig.
+    unfold val_diff_zero in eq_val_diff_z_arg2. 
+    destruct (follow_in_smap arg2 idx sb) as [fsmv|] eqn: eq_follow_arg2; try discriminate.
+    destruct fsmv as [svm] eqn: eq_fsmv.
+    destruct svm as [val2|pushtagv|label args'|offset smem|key' sstrg|
+    offset size smem] eqn: eq_svm; try discriminate.
+    destruct val2 as [v2|_a|_b] eqn: eq_val2; try discriminate.
+    rewrite -> Bool.negb_true_iff in  eq_val_diff_z_arg2.
+
+    rewrite -> eq_maxid in eval_arg2.
+    simpl in eval_arg2.
+    rewrite -> eq_follow_arg2 in eval_arg2.
+    injection eval_arg2 as eq_varg2_v2.
+    rewrite <- eq_varg2_v2 in Heval_orig.
+    pose proof (evm_jumpi_not_zero exts varg1 v2 eq_val_diff_z_arg2) as Hjumpi.
+    simpl in Hjumpi. injection Heval_orig as Heval_orig.
+    rewrite -> Hjumpi in Heval_orig.
     rewrite <- Heval_orig.
     
     unfold eval_sstack_val.
     rewrite <- eval_sstack_val'_freshvar.
-    apply eval_sstack_val'_preserved_when_depth_extended in eval_arg1.
-    apply eval'_maxidx_indep with (n:=idx).
+    apply eval_sstack_val'_preserved_when_depth_extended.
+    rewrite -> eval'_maxidx_indep_eq with (m:=idx).
     assumption.
-  + (* arg2 ~/~ WOne *)
-    injection Hoptm_sbinding as eq_val' _. 
+  + (* arg2 = WZero *)
+    injection Hoptm_sbinding as eq_val' _.
     rewrite <- eq_val'.
     assumption.
 Qed.
 
-
-End Opt_div_one.
+End Opt_jumpi_eval.
