optimizations/exp_zero_x.v
@@ -99,18 +99,18 @@ opt_smapv_valid_snd optimize_exp_zero_x_sbinding.
 Proof.
 unfold opt_smapv_valid_snd.
 intros ctx n fcmp sb val val' flag.
-intros Hvalid_smapv_val Hvalid_sb Hoptm_eq_zero_sbinding.
-unfold optimize_exp_zero_x_sbinding in Hoptm_eq_zero_sbinding.
+intros _ _ Hvalid_smapv_val Hvalid_sb Hoptm_sbinding.
+unfold optimize_exp_zero_x_sbinding in Hoptm_sbinding.
 destruct (val) as [basicv|pushtagv|label args|offset smem|key sstrg|
-  offset size smem] eqn: eq_val; try inject_rw Hoptm_eq_zero_sbinding eq_val'.
-destruct label eqn: eq_label; try inject_rw Hoptm_eq_zero_sbinding eq_val'.
+  offset size smem] eqn: eq_val; try inject_rw Hoptm_sbinding eq_val'.
+destruct label eqn: eq_label; try inject_rw Hoptm_sbinding eq_val'.
 (* EXP *)
-destruct args as [|arg1 r1]; try inject_rw Hoptm_eq_zero_sbinding eq_val'.
-destruct r1 as [|arg2 r2]; try inject_rw Hoptm_eq_zero_sbinding eq_val'.
-destruct r2; try inject_rw Hoptm_eq_zero_sbinding eq_val'.
+destruct args as [|arg1 r1]; try inject_rw Hoptm_sbinding eq_val'.
+destruct r1 as [|arg2 r2]; try inject_rw Hoptm_sbinding eq_val'.
+destruct r2; try inject_rw Hoptm_sbinding eq_val'.
 destruct (fcmp ctx arg1 (Val WZero) n sb n sb  evm_stack_opm)
-    eqn: eq_fcmp_arg1; try inject_rw Hoptm_eq_zero_sbinding eq_val'.
-injection Hoptm_eq_zero_sbinding as eq_val' eq_flag.
+    eqn: eq_fcmp_arg1; try inject_rw Hoptm_sbinding eq_val'.
+injection Hoptm_sbinding as eq_val' eq_flag.
 rewrite <- eq_val'.
 simpl in Hvalid_smapv_val. unfold valid_stack_op_instr in Hvalid_smapv_val.
 simpl in Hvalid_smapv_val.
