optimizations/shr_zero_x.v
@@ -105,7 +105,7 @@ opt_smapv_valid_snd optimize_shr_zero_x_sbinding.
 Proof.
 unfold opt_smapv_valid_snd.
 intros ctx n fcmp sb val val' flag.
-intros Hvalid_smapv_val Hvalid Hoptm_sbinding.
+intros _ _ Hvalid_smapv_val Hvalid Hoptm_sbinding.
 unfold optimize_shr_zero_x_sbinding in Hoptm_sbinding.
 destruct (val) as [basicv|pushtagv|label args|offset smem|key sstrg|
   offset size smem] eqn: eq_val; 
