optimizations/strg_solver.v
@@ -1,0 +1,199 @@
+Require Import bbv.Word.
+Require Import Nat.
+Require Import Coq.NArith.NArith.
+
+Require Import Coq.Logic.FunctionalExtensionality.
+
+Require Import FORVES2.constants.
+Import Constants.
+
+Require Import FORVES2.symbolic_state.
+Import SymbolicState.
+
+Require Import FORVES2.symbolic_state_eval.
+Import SymbolicStateEval.
+
+Require Import FORVES2.symbolic_state_cmp.
+Import SymbolicStateCmp.
+
+Require Import FORVES2.valid_symbolic_state.
+Import ValidSymbolicState.
+
+Require Import FORVES2.execution_state.
+Import ExecutionState.
+
+Require Import FORVES2.stack_operation_instructions.
+Import StackOpInstrs.
+
+Require Import FORVES2.program.
+Import Program.
+
+Require Import FORVES2.symbolic_state_cmp_impl.
+Import SymbolicStateCmpImpl.
+
+Require Import FORVES2.symbolic_state_eval_facts.
+Import SymbolicStateEvalFacts.
+
+Require Import FORVES2.valid_symbolic_state.
+Import ValidSymbolicState.
+
+Require Import FORVES2.misc.
+Import Misc.
+
+Require Import FORVES2.eval_common.
+Import EvalCommon.
+
+Require Import FORVES2.concrete_interpreter.
+Import ConcreteInterpreter.
+
+Require Import FORVES2.optimizations_def.
+Import Optimizations_Def.
+
+Require Import FORVES2.optimizations_common.
+Import Optimizations_Common.
+
+Require Import FORVES2.storage_ops_solvers.
+Import StorageOpsSolvers.
+
+Require Import FORVES2.storage_ops_solvers_impl.
+Import StorageOpsSolversImpl.
+
+Require Import FORVES2.storage_ops_solvers_impl_soundness.
+Import StorageOpsSolversImplSoundness.
+
+Require Import FORVES2.constraints.
+Import Constraints.
+
+Require Import List.
+Import ListNotations.
+
+
+Module Opt_strg_solver.
+
+Definition strg_solver_applied (val1 val2: smap_value) : bool :=
+(* If sload_solver does not return SymSLOAD or the symbolic storages have 
+   different lengths, then optimized *)
+match val1, val2 with
+| SymSLOAD skey sstrg, SymSLOAD skey' sstrg' => negb (length sstrg =? length sstrg')
+| _, _ => true
+end.
+
+(* Storage solver 
+  SymSLOAD skey sstrg --> smapv
+     if basic_sload_solver (SymSLOAD skey sstrg) = smapv
+*)
+Definition optimize_strg_solver_sbinding : opt_smap_value_type :=
+fun (val: smap_value) =>
+fun (fcmp: sstack_val_cmp_t) =>
+fun (sb: sbindings) =>
+fun (maxid: nat) =>
+fun (ctx: constraints) =>
+fun (ops: stack_op_instr_map) => 
+match val with
+| SymSLOAD skey sstrg => 
+     let val' := (basic_sload_solver (fun _:nat => fcmp) ctx skey sstrg  
+                   (SymMap maxid sb) ops) in
+     let flag := strg_solver_applied val val' in
+     (val', flag)
+| _ => (val, false)
+end.
+(* TODO:
+- CHECK if is better to pass the whole smap ==> adapt 60 files
+- CHECK if maxid is correctly computed
+- CHECK if (fun _:nat => fcmp) is an appropiate value of sstack_val_cmp_ext_1_t
+    (fcmp is already instantiated with the right maxid, so the lambda receives a
+     dummy maxid and discards it)
+*)
+
+
+Lemma optimize_strg_solver_sbinding_smapv_valid:
+opt_smapv_valid_snd optimize_strg_solver_sbinding.
+Proof.
+unfold opt_smapv_valid_snd.
+intros ctx n fcmp sb val val' flag.
+intros Hsafe_sstack_val_cmp His_sat Hvalid_smapv_val Hvalid_sb Hoptm_sbinding.
+unfold optimize_strg_solver_sbinding in Hoptm_sbinding.
+destruct (val) as [basicv|pushtagv|label args|offset smem|skey sstrg|
+  offset size smem] eqn: eq_val; try (
+    injection Hoptm_sbinding as eq_val' _;
+    rewrite <- eq_val';
+    assumption).
+(* SymSLOAD skey sstrg *)
+pose proof (basic_sload_solver_snd (fun _ : nat => fcmp)
+    (safe_fcm_ext_1 fcmp Hsafe_sstack_val_cmp)).
+unfold sload_solver_snd in H.
+destruct H as [Hsolver_valid _].
+unfold sload_solver_valid_res in Hsolver_valid.
+specialize Hsolver_valid with (m:=SymMap n sb)(sstrg:=sstrg)(skey:=skey)
+  (ctx:=ctx)(smv:=val')(ops:=evm_stack_opm).
+simpl in Hsolver_valid.
+unfold valid_smap_value in Hvalid_smapv_val.
+destruct Hvalid_smapv_val as [Hvalid_sstack_val Hvalid_sstorage].
+injection Hoptm_sbinding as eq_basic_mload_solver _.
+pose proof (Hsolver_valid His_sat Hvalid_sstorage Hvalid_sstack_val 
+  eq_basic_mload_solver).
+assumption.
+Qed.
+
+
+Lemma optimize_strg_solver_sbinding_snd:
+opt_sbinding_snd optimize_strg_solver_sbinding.
+Proof.
+unfold opt_sbinding_snd.
+intros val val' fcmp sb maxidx ctx idx flag Hsafe_sstack_val_cmp
+  Hvalid His_sat Hoptm_sbinding.
+split.
+- (* valid_sbindings *)
+  apply valid_bindings_snd_opt with (val:=val)(opt:=optimize_strg_solver_sbinding)
+    (fcmp:=fcmp)(flag:=flag)(ctx:=ctx); try assumption.
+  apply optimize_strg_solver_sbinding_smapv_valid. 
+
+- (* evaluation is preserved *) 
+  intros model mem strg exts v His_model Heval_orig.
+  unfold optimize_strg_solver_sbinding in Hoptm_sbinding.
+  destruct val as [vv|vv|label args|offset smem|skey sstrg|offset size smem]
+    eqn: eq_val; try inject_rw Hoptm_sbinding eq_val'.
+  (* SymSLOAD skey sstrg *)
+  injection Hoptm_sbinding as eq_basic_solver eq_flag.
+  pose proof (basic_sload_solver_snd (fun _ : nat => fcmp)
+      (safe_fcm_ext_1 fcmp Hsafe_sstack_val_cmp)).
+  unfold sload_solver_snd in H.
+  destruct H as [Hsolver_valid Hsolver_correct].
+  unfold sload_solver_correct_res in Hsolver_correct.
+  specialize Hsolver_correct with (m := SymMap idx sb)(sstrg:=sstrg)
+    (skey:=skey)(ctx:=ctx)(smv:=val')
+    (ops:=evm_stack_opm)(idx1:=idx)(m1:=SymMap maxidx
+    ((idx,val')::sb)).
+  unfold valid_bindings in Hvalid.
+  destruct Hvalid as [eq_maxidx_idx [eq_valid_smapv eq_valid_bindings]].
+  fold valid_bindings in eq_valid_bindings.
+  unfold valid_smap in Hsolver_correct.
+  simpl in Hsolver_correct.
+
+  pose proof (Hsolver_correct His_sat eq_valid_bindings) as Hsolver_correct.
+  unfold valid_smap_value in eq_valid_smapv.
+  destruct eq_valid_smapv as [eq_valid_offset eq_valid_smem].
+  rewrite -> eq_maxidx_idx in Hsolver_correct.
+  pose proof (Hsolver_correct eq_valid_smem eq_valid_offset eq_basic_solver) 
+    as Hsolver_correct.
+  assert ((idx, SymMap (S idx) ((idx, val') :: sb)) =
+          (idx, SymMap (S idx) ((idx, val') :: sb))) as eq_smaps; 
+      try reflexivity.
+  pose proof (Hsolver_correct eq_smaps) as Hsolver_correct.
+  destruct Hsolver_correct as [idx2 [m2 [eq_m2 HH]]].
+  injection eq_m2 as eq_idx2 eq_m2.
+  specialize HH with (model:=model)(mem:=mem)(strg:=strg)(exts:=exts).
+  pose proof (HH His_model) as HH.
+  destruct HH as [vv [Heval1 Heval2]].
+  rewrite <- eq_idx2 in Heval2.
+  rewrite <- eq_m2 in Heval2.
+  simpl in Heval2.
+  rewrite <- eq_maxidx_idx in Heval2.
+  rewrite -> Heval_orig in Heval2.
+  rewrite -> Heval2.
+  rewrite -> eq_maxidx_idx.
+  assumption.
+Qed.
+
+
+End Opt_strg_solver.
